B_Unification/sve.v
@@ -87,19 +87,26 @@ Proof.
   apply make_poly_is_poly.
 Qed.
 
-Lemma already_poly : forall p,
-  NoDup p ->
-  (forall m, In m p -> is_mono m) ->
-  nodup_cancel mono_eq_dec (map make_mono p) = p.
-Proof.
-Admitted.
-
-Lemma ugh : forall x p a,
-  is_poly (a :: p) ->
+Lemma NoDup_map_remove : forall x p,
+  is_poly p ->
   (forall m, In m p -> In x m) ->
-  NoDup (remove var_eq_dec x a :: map (remove var_eq_dec x) p).
+  NoDup (map (remove var_eq_dec x) p).
 Proof.
-Admitted.
+  intros x p Hp Hx. induction p.
+  - simpl. auto.
+  - simpl. apply NoDup_cons.
+    + intro. apply in_map_iff in H. destruct H as [y []]. assert (y = a).
+      * apply poly_cons in Hp. destruct Hp. unfold is_poly in H1. destruct H1.
+        apply H3 in H0. apply (remove_Sorted_eq _ var_eq_dec x lt); auto.
+        -- apply NoDup_VarSorted in H0. auto.
+        -- apply NoDup_VarSorted in H2. auto.
+      * rewrite H1 in H0. unfold is_poly in Hp. destruct Hp.
+        apply NoDup_MonoSorted in H2 as H4. apply NoDup_cons_iff in H4 as []. 
+        contradiction.
+    + apply IHp.
+      * apply poly_cons in Hp. apply Hp.
+      * intros m H. apply Hx. intuition.
+Qed.
 
 Lemma elim_var_map_remove_Permutation : forall p x,
   is_poly p ->
@@ -107,15 +114,41 @@ Lemma elim_var_map_remove_Permutation : forall p x,
   Permutation (elim_var x p)
               (map (remove var_eq_dec x) p).
 Proof.
-  intros p x H H0. induction p.
+  intros p x H H0. destruct p as [|a p].
   - simpl. unfold elim_var, make_poly, MonoSort.sort. auto.
   - simpl. unfold elim_var. simpl. unfold make_poly. pose (MonoSort.Permuted_sort (nodup_cancel mono_eq_dec (map make_mono (remove var_eq_dec x a :: map (remove var_eq_dec x) p)))).
     assert (Permutation (nodup_cancel mono_eq_dec (map make_mono (remove var_eq_dec x a :: map (remove var_eq_dec x) p))) (remove var_eq_dec x a :: map (remove var_eq_dec x) p)).
-    + clear p0. rewrite already_poly.
+    + clear p0. rewrite unsorted_poly.
       * apply Permutation_refl.
-      * apply ugh; auto. intros m Hin. apply H0; intuition.
-      * intros m Hin. admit.
+      * rewrite <- map_cons. apply NoDup_map_remove; auto.
+      * apply poly_cons in H. intros m Hin. destruct Hin.
+        -- rewrite <- H1. apply remove_is_mono. apply H.
+        -- apply in_map_iff in H1 as [y []]. rewrite <- H1. apply remove_is_mono.
+           destruct H. unfold is_poly in H. destruct H. apply H4. auto.
     + apply Permutation_sym in p0. apply (Permutation_trans p0 H1).
+Qed.
+
+Lemma concat_map : forall {A B:Type} (f:A->B) (l:list A),
+  concat (map (fun a => [f a]) l) = map f l.
+Proof.
+  intros A B f l. induction l.
+  - auto.
+  - simpl. f_equal. apply IHl.
+Qed.
+
+Lemma NoDup_map_app : forall x l,
+  is_poly l ->
+  (forall m, In m l -> ~ In x m) ->
+  NoDup (map make_mono (map (fun a : list var => a ++ [x]) l)).
+Proof.
+  intros x l Hp Hin. induction l.
+  - simpl. auto.
+  - simpl. apply NoDup_cons.
+    + intros H. rewrite map_map in H. apply in_map_iff in H as [m []]. assert (a=m).
+      * apply Permutation_Sorted_mono_eq; admit.
+      * rewrite <- H1 in H0. unfold is_poly in Hp. destruct Hp.
+        apply NoDup_MonoSorted in H2. apply NoDup_cons_iff in H2 as []. contradiction.
+    + apply IHl. apply poly_cons in Hp. apply Hp. intros m H. apply Hin. intuition.
 Admitted.
 
 Lemma mulPP_Permutation : forall x a0 l,
@@ -127,14 +160,15 @@ Proof.
   pose (MonoSort.Permuted_sort (nodup_cancel mono_eq_dec
         (map make_mono ((a0 ++ [x]) :: concat (map (fun a : list var => [a ++ [x]]) l))))).
   apply Permutation_sym in p. apply (Permutation_trans p). simpl map.
-  assert ((nodup_cancel mono_eq_dec
-     (make_mono (a0 ++ [x]) :: map make_mono (concat (map (fun a : list var => [a ++ [x]]) l)))) = 
-     (make_mono (a0 ++ [x]) :: map make_mono (concat (map (fun a : list var => [a ++ [x]]) l)))).
-     admit.
-  rewrite H. apply perm_skip. clear p; clear H. apply Permutation_trans with (l':=(nodup_cancel mono_eq_dec (map make_mono (concat (map (fun a : list var => [a ++ [x]]) l))))).
-  - admit.
-  - apply MonoSort.Permuted_sort.
-Admitted.
+  rewrite no_nodup_cancel_NoDup; clear p.
+  - apply perm_skip. apply Permutation_trans with (l':=(nodup_cancel mono_eq_dec (map make_mono (concat (map (fun a : list var => [a ++ [x]]) l))))).
+    + rewrite no_nodup_cancel_NoDup; auto. rewrite concat_map. apply NoDup_map_app.
+      apply poly_cons in Hp. apply Hp. intros m H. apply Hx. intuition.
+    + apply MonoSort.Permuted_sort.
+  - rewrite <- map_cons. rewrite concat_map.
+    rewrite <- map_cons with (f:=(fun a : list var => a ++ [x])).
+    apply NoDup_map_app; auto.
+Qed.
 
 Lemma mulPP_map_app_permutation : forall (x:var) (l l' : poly),
   is_poly l ->
